proof/old_system/uni/algo_worklist/prop_basic.v
@@ -15,3 +15,147 @@ Theorem a_mono_typ_wf : forall aE A,
 Proof.
   intros. induction H; auto.
 Qed.
+
+(* Fixpoint subst_tvar_in_aworklist *)
+
+(* Theorem a_wl_red_rename_tvar : forall Γ1 Γ2 X b X',
+  awl_app Γ2 (aworklist_constvar Γ1 X b) ⟶ᵃʷ⁎⋅ ->
+  awl_app (subst_tvar_in_aworklist (typ_var_f X') X Γ2) (aworklist_constvar Γ1 X' b) ⟶ᵃʷ⁎⋅.
+Proof.
+  intros. induction Γ2.
+  - simpl in *. destruct b.
+    + dependent destruction H. econstructor; auto.
+    + dependent destruction H. econstructor; auto.
+    + dependent destruction H. econstructor; auto.
+    + dependent destruction H. econstructor; auto.
+  - simpl in *. destruct ab; try dependent destruction H.
+    apply a_wl_red__gc_var; auto.
+  - admit.
+Admitted. *)
+
+(* Theorem a_wl_red_rename_tvar' : forall Γ1 Γ2 X b X',
+  awl_app Γ2 (aworklist_constvar Γ1 X b) ⟶ᵃʷ⁎⋅ ->
+  awl_app (subst_tvar_in_aworklist (typ_var_f X') X Γ2) (aworklist_constvar Γ1 X' b) ⟶ᵃʷ⁎⋅.
+Proof.
+  intros. dependent induction H.
+  - admit.
+  -
+  - simpl in *. destruct ab; try dependent destruction H.
+    apply a_wl_red__gc_var; auto.
+  - admit.
+  -
+
+  
+Qed.
+ *)
+
+Hint Constructors a_wl_red : Hdb_a_wl_red_basic.
+Hint Constructors apply_cont : Hdb_a_wl_red_basic.
+Hint Constructors aworklist_subst : Hdb_a_wl_red_basic.
+
+
+Lemma apply_cont_rename : forall c A w X X',
+  apply_cont c A w ->
+  apply_cont (subst_tvar_in_cont (typ_var_f X') X c) (subst_tvar_in_typ (typ_var_f X') X A) 
+    (subst_tvar_in_work (typ_var_f X') X w).
+Proof.
+  intros. induction H; simpl; try solve [simpl; eauto with Hdb_a_wl_red_basic].
+Qed.
+
+Fixpoint subst_tvar_in_etvar_list (X' X: typvar) (E:list typvar) :=
+  match E with 
+  | nil => nil
+  | X0 :: E' => (if X0 == X then X' else X0) :: (subst_tvar_in_etvar_list X X' E') 
+  end.
+
+
+Fixpoint rename_tvar_in_aworklist (X' X:typvar) (Γ:aworklist) {struct Γ} : aworklist :=
+  match Γ with
+  | aworklist_empty => aworklist_empty 
+  | (aworklist_consvar Γ' x b) => aworklist_consvar (rename_tvar_in_aworklist X' X Γ') x (subst_tvar_in_abind (typ_var_f X') X b)
+  | (aworklist_constvar Γ' X0 b) => aworklist_constvar (rename_tvar_in_aworklist X' X Γ') (if X0 == X then X' else X0) (subst_tvar_in_abind (typ_var_f X') X b)
+  | (aworklist_conswork Γ' w) => aworklist_conswork (rename_tvar_in_aworklist X' X Γ') (subst_tvar_in_work (typ_var_f X') X w)
+end.
+
+Lemma worklist_subst_rename : forall Γ X X' A E Γ1 Γ2,
+  aworklist_subst Γ X A E Γ1 Γ2 -> 
+  aworklist_subst (rename_tvar_in_aworklist X' X Γ) X' ({` X' /ᵗ X} A) 
+      (subst_tvar_in_etvar_list X' X E) (rename_tvar_in_aworklist X' X Γ1) (rename_tvar_in_aworklist X' X Γ2).
+Proof.
+  intros. induction H.
+  - simpl. admit.
+  - admit.
+  - 
+Admitted.
+
+Theorem a_wl_red_rename_tvar : forall Γ X X',
+  Γ ⟶ᵃʷ⁎⋅ ->
+  (rename_tvar_in_aworklist X' X Γ) ⟶ᵃʷ⁎⋅.
+Proof with eauto with Hdb_a_wl_red_basic.
+  intros. dependent induction H; try solve [simpl; eauto with Hdb_a_wl_red_basic].
+  - admit. 
+  - simpl.
+    eapply a_wl_red__sub_alll with (L:=L `union` singleton X).
+    + admit.
+    + admit.
+    + admit.
+    + intros. simpl in *. inst_cofinites_with X0.
+      rewrite typ_subst_open_comm...
+      unfold eq_dec in H3.
+      destruct (EqDec_eq_of_X X0 X) in H3...
+      admit.
+  - simpl.
+    eapply a_wl_red__sub_all with (L:=L `union` singleton X).
+    intros. inst_cofinites_with X0.
+    simpl in H0.
+    rewrite typ_subst_open_comm...
+    rewrite typ_subst_open_comm...
+    admit.
+  - simpl. 
+    destruct (X0 == X).
+    + subst.
+      eapply a_wl_red__sub_arrow1 with (L:=L)... admit.
+      admit.
+      intros.
+      inst_cofinites_with X1. inst_cofinites_with X2.
+      admit.
+    + eapply a_wl_red__sub_arrow1 with (L:=L)... admit.
+      admit.
+      intros.
+      inst_cofinites_with X1. inst_cofinites_with X2.
+      admit.
+  - admit.
+  - simpl. destruct (X0 == X).
+    + subst.
+      eapply a_wl_red__sub_etvarmono1; auto. admit.
+      admit.
+      admit.
+      admit.
+    + eapply a_wl_red__sub_etvarmono1; auto. admit.
+      admit.
+      admit.
+      admit.
+  - simpl. destruct (X0 == X).
+    + subst.
+      eapply a_wl_red__sub_etvarmono2; auto. admit.
+       admit.
+       admit.
+       admit.
+    + eapply a_wl_red__sub_etvarmono2; auto. admit.
+      admit.
+      admit.
+      admit.
+  - admit.
+  - admit.
+  - admit.
+  - admit.
+  - admit.
+  - admit.
+  - admit.
+  - admit.
+  - simpl in *. 
+    eapply a_wl_red__inftapp_all.
+    rewrite <- subst_tvar_in_typ_open_typ_wrt_typ...
+  - simpl. 
+    eapply apply_cont_rename with (X:=X) (X':=X') in H...
+Admitted.
